Test/Tactic.lean
@@ -23,97 +23,116 @@ Demonstrate that SlimCheck can handle the basic types from core:
 - Array
 -/
 
-/-- error: Found problems! -/
+
+/-- error: Found a counter-example! -/
 #guard_msgs in
 example (a b : Sum Nat Nat) : a = b := by
   slim_check (config := {quiet := true})
 
-/-- error: Found problems! -/
+/-- error: Found a counter-example! -/
 #guard_msgs in
 example (a b : Σ n : Nat, Nat) : a.fst = b.snd := by
   slim_check (config := {quiet := true})
 
-/-- error: Found problems! -/
+/-- error: Found a counter-example! -/
 #guard_msgs in
 example (a b : Unit) : a ≠ b := by
   slim_check (config := {quiet := true})
 
-/-- error: Found problems! -/
+/-- error: Found a counter-example! -/
 #guard_msgs in
 example (x y : Nat × Unit) : x = y := by
   slim_check (config := {quiet := true})
 
-/-- error: Found problems! -/
+/-- error: Found a counter-example! -/
 #guard_msgs in
 example (a b : Bool) : a = b :=  by
   slim_check (config := {quiet := true})
 
-/-- error: Found problems! -/
+/-- error: Found a counter-example! -/
 #guard_msgs in
 example (a b c : Nat) : a + (b - c) = (a + b) - c := by
   slim_check (config := {quiet := true})
 
-/-- error: Found problems! -/
+/-- error: Found a counter-example! -/
 #guard_msgs in
 example (a : Fin (n + 1)) : a + 1 > a := by
   slim_check (config := {quiet := true})
 
-/-- error: Found problems! -/
+/-- error: Found a counter-example! -/
 #guard_msgs in
 example (a : BitVec n) : a + 1 > a := by
   slim_check (config := {quiet := true})
 
-/-- error: Found problems! -/
+/-- error: Found a counter-example! -/
 #guard_msgs in
 example (a : UInt8) : a - 1 < a := by
   slim_check (config := {quiet := true})
 
-/-- error: Found problems! -/
+/-- error: Found a counter-example! -/
 #guard_msgs in
 example (a : UInt16) : a - 1 < a := by
   slim_check (config := {quiet := true})
 
-/-- error: Found problems! -/
+/-- error: Found a counter-example! -/
 #guard_msgs in
 example (a : UInt32) : a - 1 < a := by
   slim_check (config := {quiet := true})
 
-/-- error: Found problems! -/
+/-- error: Found a counter-example! -/
 #guard_msgs in
 example (a : UInt64) : a - 1 < a := by
   slim_check (config := {quiet := true})
 
-/-- error: Found problems! -/
+/-- error: Found a counter-example! -/
 #guard_msgs in
 example (a : USize) : a - 1 < a := by
   slim_check (config := {quiet := true})
 
-/-- error: Found problems! -/
+/-- error: Found a counter-example! -/
 #guard_msgs in
 example (a : Char) : a ≠ a := by
   slim_check (config := {quiet := true})
 
-/-- error: Found problems! -/
+/-- error: Found a counter-example! -/
 #guard_msgs in
 example (a : Option Char) : a ≠ a := by
   slim_check (config := {quiet := true})
 
-/-- error: Found problems! -/
+/-- error: Found a counter-example! -/
 #guard_msgs in
 example (xs ys : List Nat) : xs.length = ys.length → xs = ys := by
   slim_check (config := {quiet := true})
 
-/-- error: Found problems! -/
+/-- error: Found a counter-example! -/
 #guard_msgs in
 example (xs ys : String) : xs.length = ys.length → xs = ys := by
   slim_check (config := {quiet := true})
 
-/-- error: Found problems! -/
+/-- error: Found a counter-example! -/
 #guard_msgs in
 example (xs ys : Array Nat) : xs.size = ys.size → xs = ys := by
   slim_check (config := {quiet := true})
 
-/-- error: Found problems! -/
+/-- error: Found a counter-example! -/
 #guard_msgs in
 example (xs : List Int) (f : Int → Int) : xs.map f = xs := by
   slim_check (config := {quiet := true})
+
+/--
+info: Unable to find a counter-example
+---
+warning: declaration uses 'sorry'
+-/
+#guard_msgs in
+example (a : Sum Nat Nat) : a = a := by
+  slim_check
+
+/--
+warning: Gave up after failing to generate values that fulfill the preconditions 100 times.
+---
+warning: declaration uses 'sorry'
+-/
+#guard_msgs in
+example (a b : Sum Nat Nat) : a ≠ a → a = b := by
+  slim_check (config := {numInst := 100})
